src/rocq/Handlers/Global.v
@@ -4,8 +4,8 @@ From Stdlib Require Import
      String.
 
 From ExtLib Require Import
-     Structures.Monads
-     Structures.Maps.
+     Structures.Maps
+     Data.Map.FMapAList.
 
 From ITree Require Import
      ITree
@@ -15,9 +15,7 @@ From ITree Require Import
      InterpFacts.
 
 From Vellvm Require Import
-     Utils.Util
-     Utils.Error
-     Utils.Tactics
+     Utilities
      Semantics.LLVMParams
      Semantics.LLVMEvents.
 
@@ -26,9 +24,7 @@ From QuickChick Require Import Show.
 Set Implicit Arguments.
 Set Contextual Implicit.
 
-Import MonadNotation.
 Import ITree.Basics.Basics.Monads.
-Open Scope string_scope.
 (* end hide *)
 
 (** * Global handler
@@ -52,26 +48,25 @@ Section Globals.
         end
       end.
 
-  (* See src/ml/Extract.v for the special handling of these operation. *)
-  Record debug_globals := mk_debug_globals {
-      globals_set : map -> unit ;
-      globals_get : unit -> map;
-    }.
+  (* (* See src/ml/Extract.v for the special handling of these operation. *) *)
+  (* Record debug_globals := mk_debug_globals { *)
+  (*     globals_set : map -> unit ; *)
+  (*     globals_get : unit -> map; *)
+  (*   }. *)
 
-  Definition globals_object : debug_globals :=
-    mk_debug_globals (fun (_:map) => tt) (fun (_:unit) => (Maps.empty : map)).
+  (* Definition globals_object : debug_globals := *)
+  (*   mk_debug_globals (fun (_:map) => tt) (fun (_:unit) => (Maps.empty : map)). *)
 
-  Definition update_globals_ref {M} `{HM: Monad M} {T} (e : GlobalE k v T) : stateT map M unit :=
-    (gs <- MonadState.get;;
-    ret (globals_object.(globals_set) gs))%monad.
- 
-  Definition handle_global_debug {E} `{FailureE -< E} : (GlobalE k v) ~> stateT map (itree E) :=
-    fun _ e =>
-      (res <- handle_global e;;
-      update_globals_ref e;;
-      ret res)%monad.
+  (* Definition update_globals_ref {M} `{HM: Monad M} {T} (e : GlobalE k v T) : stateT map M unit := *)
+  (*   (gs <- MonadState.get;; *)
+  (*    ret (globals_object.(globals_set) gs))%monad. *)
+  
+  (* Definition handle_global_debug {E} `{FailureE -< E} : (GlobalE k v) ~> stateT map (itree E) := *)
+  (*   fun _ e => *)
+  (*     (res <- handle_global e;; *)
+  (*     update_globals_ref e;; *)
+  (*     ret res)%monad. *)
 
-  Open Scope monad_scope.
   Section PARAMS.
     Variable (E F G H : Type -> Type).
     Context `{FailureE -< G}.
@@ -87,7 +82,7 @@ Section Globals.
     Definition G_trigger {M} : forall R , G R -> (stateT M (itree Effout) R) :=
       fun R e m => r <- trigger e ;; ret (m, r).
 
-    Definition interp_global_h := (case_ E_trigger (case_ F_trigger (case_ handle_global_debug G_trigger))).
+    Definition interp_global_h := (case_ E_trigger (case_ F_trigger (case_ handle_global(* handle_global_debug *) G_trigger))).
     Definition interp_global  : itree Effin ~> stateT map (itree Effout) :=
       interp_state interp_global_h.
 
