src/rocq/Handlers/MemPropT.v
@@ -1,28 +1,13 @@
-From Stdlib Require Import
-     Strings.String
-     ZArith.
-
-From ExtLib Require Import
-     Structures.Monad.
-
 From ITree Require Import
-     ITree
-     Basics.Basics
-     Eq.Eqit
-     Events.StateFacts
-     Events.State.
+  ITree
+  Basics.Basics
+  Eq.Eqit
+  Events.StateFacts
+  Events.State.
 
-From Vellvm Require Import Error.
-
-From Vellvm.Utils Require Import
-     MonadEq1Laws
-     PropT
-     Raise
-     Tactics
-     Inhabited.
-
-From Vellvm.Handlers.MemoryModules Require Import
-     Within.
+From Vellvm Require Import
+  Utilities
+  Propositional.Within.
 
 From Vellvm.Semantics Require Import
   LLVMEvents.
@@ -68,7 +53,7 @@ Import Morphisms.
     (*   (ma : M A) : stateT MemState (itree E) A; *)
 
 Definition MemPropT (MemState : Type) (X : Type) : Type
-  := MemState -> err_ub_oom (MemState * X)%type -> Prop.
+  := MemState -> EOB (MemState * X)%type -> Prop.
 
 (* Instance MemPropT_Monad : Monad MemPropT. *)
 (* Proof. *)
@@ -108,36 +93,30 @@ Proof.
   - (* ret *)
     refine (fun _ v s r =>
               match r with
-              | ERR_UB_OOM (mkEitherT (mkEitherT (mkEitherT (mkIdent r)))) =>
-                  match r with
-                  | inl (OOM_message x) => False
-                  | inr (inl (UB_message x)) => False
-                  | inr (inr (inl (ERR_message x))) => False
-                  | inr (inr (inr (s',r'))) => s' = s /\ r' = v
-                  end
+              | raise_oom   x => False
+              | raise_ub    x => False
+              | raise_error x => False
+              | raise_ret (s',r') => s' = s /\ r' = v
               end).
   - (* bind *)
     refine (fun A B ma amb sa r =>
               match r with
-              | ERR_UB_OOM (mkEitherT (mkEitherT (mkEitherT (mkIdent r)))) =>
-                  match r with
-                  | inl (OOM_message msg') =>
-                      (ma sa (raise_oom msg') \/
-                         (exists sab a, ma sa (ret (sab, a)) /\
-                                     (amb a sab (raise_oom msg'))))
-                  | inr (inl (UB_message msg')) =>
-                      (ma sa (raise_ub msg') \/
-                         (exists sab a, ma sa (ret (sab, a)) /\
-                                     (amb a sab (raise_ub msg'))))
-                  | inr (inr (inl (ERR_message msg'))) =>
-                      (ma sa (raise_error msg') \/
-                         (exists sab a, ma sa (ret (sab, a)) /\
-                                     (amb a sab (raise_error msg'))))
-                  | inr (inr (inr (s',r'))) =>
-                      exists sab a,
-                      ma sa (ret (sab, a)) /\
-                        amb a sab (ret (s', r'))
-                  end
+              | raise_oom msg' =>
+                  (ma sa (raise_oom msg') \/
+                     (exists sab a, ma sa (ret (sab, a)) /\
+                                 (amb a sab (raise_oom msg'))))
+              | raise_ub msg' =>
+                  (ma sa (raise_ub msg') \/
+                     (exists sab a, ma sa (ret (sab, a)) /\
+                                 (amb a sab (raise_ub msg'))))
+              | raise_error msg' =>
+                  (ma sa (raise_error msg') \/
+                     (exists sab a, ma sa (ret (sab, a)) /\
+                                 (amb a sab (raise_error msg'))))
+              | raise_ret (s',r') =>
+                  exists sab a,
+                  ma sa (ret (sab, a)) /\
+                    amb a sab (ret (s', r'))
               end).
 Defined.
 
@@ -146,7 +125,7 @@ Proof.
   unfold Eq1.
   intros A m1 m2.
   unfold MemPropT in *.
-  exact (forall (ms : MemState) (x : err_ub_oom (MemState * A)),
+  exact (forall (ms : MemState) (x : EOB (MemState * A)),
             m1 ms x <-> m2 ms x).
 Defined.
 
@@ -177,56 +156,56 @@ Proof.
       intros M.
     +
       (* TODO: Move to Error.v *)
-      destruct_err_ub_oom x0; firstorder; subst; firstorder.
+      destruct x0; firstorder; subst; firstorder.
       repeat break_match_hyp.
       destruct M as (sab & a & (EQ1 & EQ2) & F); subst.
       auto.
-    + destruct_err_ub_oom x0; firstorder.
-      destruct x1. exists ms. exists x. firstorder.
+    + destruct x0; firstorder.
+      destruct x0. exists ms. exists x. firstorder.
   - intros A x.
     cbn.
     unfold eq1, MemPropT_Eq1 in *.
     split;
       intros M.
-    + destruct_err_ub_oom x0; firstorder; subst; firstorder.
+    + destruct x0; firstorder; subst; firstorder.
       repeat break_match_hyp.
       destruct M as (sab & a' & F & (EQ1 & EQ2)); subst.
       auto.
-    + destruct_err_ub_oom x0; firstorder.
-      destruct x1. exists m. exists a. firstorder.
+    + destruct x0; firstorder.
+      destruct x0. exists m. exists a. firstorder.
   - intros A B C x f g.
     cbn.
     unfold eq1, MemPropT_Eq1 in *.
     split;
       intros M.
-    + destruct_err_ub_oom x0; firstorder; subst; firstorder.
-      * right. exists x3. exists x4. firstorder.
-      * right. exists x3. exists x4. firstorder.
-      * right. exists x3. exists x4. firstorder.
-      * destruct x1.
+    + destruct x0; firstorder; subst; firstorder.
+      * right. exists x2. exists x3. firstorder.
+      * right. exists x2. exists x3. firstorder.
+      * right. exists x2. exists x3. firstorder.
+      * destruct x0.
         destruct M as (sab & b & ((sab' & a' & (x' & f')) & g')); subst.
         eexists. eexists. eauto.
-    + destruct_err_ub_oom x0; firstorder; subst; firstorder.
+    + destruct x0; firstorder; subst; firstorder.
       * right. eexists. eexists. eauto.
       * right. eexists. eexists. eauto.
       * right. eexists. eexists. eauto.
-      * destruct x1.
+      * destruct x0.
         destruct M as (sab & a' & Hx & (sab' & b' & (f' & g'))); subst.
         eexists. eexists. eauto.
   - repeat red. intros.
     split; cbn; intros.
-    + destruct_err_ub_oom x1; firstorder; subst; firstorder.
-      * right. exists x2. exists x3. split. apply H. assumption. apply H0. assumption.
-      * right. exists x2. exists x3. split. apply H. assumption. apply H0. assumption.
-      * right. exists x2. exists x3. split. apply H. assumption. apply H0. assumption.
-      * destruct x2.
+    + destruct x1; firstorder; subst; firstorder.
+      * right. exists x1. exists x2. split. apply H. assumption. apply H0. assumption.
+      * right. exists x1. exists x2. split. apply H. assumption. apply H0. assumption.
+      * right. exists x1. exists x2. split. apply H. assumption. apply H0. assumption.
+      * destruct x1.
         destruct H1 as (sab & a & (HX & HY)).
         exists sab. exists a. split. apply H. assumption. apply H0. assumption.
-    + destruct_err_ub_oom x1; firstorder; subst; firstorder.
-      * right. exists x2. exists x3. split. apply H. assumption. apply H0. assumption.
-      * right. exists x2. exists x3. split. apply H. assumption. apply H0. assumption.
-      * right. exists x2. exists x3. split. apply H. assumption. apply H0. assumption.
-      * destruct x2.
+    + destruct x1; firstorder; subst; firstorder.
+      * right. exists x1. exists x2. split. apply H. assumption. apply H0. assumption.
+      * right. exists x1. exists x2. split. apply H. assumption. apply H0. assumption.
+      * right. exists x1. exists x2. split. apply H. assumption. apply H0. assumption.
+      * destruct x1.
         destruct H1 as (sab & a & (HX & HY)).
         exists sab. exists a. split. apply H. assumption. apply H0. assumption.
 Qed.
@@ -238,7 +217,7 @@ Proof.
   - (* get_mem_state *)
     unfold MemPropT.
     intros ms res.
-    destruct res as [[[[[[[oom_res] | [[ub_res] | [[err_res] | [ms' a]]]]]]]]] eqn:Hres.
+    destruct res.
     + (* OOM *)
       exact False.
     + (* UB *)
@@ -246,253 +225,205 @@ Proof.
     + (* Error *)
       exact False.
     + (* Success *)
+      destruct x as [ms' a].
       exact (ms = ms' /\ a = ms).
   - (* put_mem_state *)
     unfold MemPropT.
     intros ms_to_put ms res.
-    destruct res as [[[[[[[oom_res] | [[ub_res] | [[err_res] | [ms' a]]]]]]]]] eqn:Hres.
+    destruct res.
     + (* OOM *)
       exact False.
     + (* UB *)
       exact False.
     + (* Error *)
       exact False.
-    + exact (ms_to_put = ms').
+    + destruct x as [ms' a].
+      exact (ms_to_put = ms').
 Defined.
 
-#[global] Instance MemPropT_RAISE_OOM {MemState : Type} : RAISE_OOM (MemPropT MemState).
-Proof.
-  split.
-  - intros A msg.
-    unfold MemPropT.
-    intros ms res.
-    destruct res as [[[[[[[oom_res] | [[ub_res] | [[err_res] | [ms' a]]]]]]]]] eqn:Hres.
-    + (* OOM *)
-      exact True. (* Don't care about particular error message, every OOM allowed. *)
-    + (* UB *)
-      exact False. (* Must run out of memory, can't UB *)
-    + (* Error *)
-      exact False. (* Must run out of memory, can't error *)
-    + (* Success *)
-      exact False. (* Must run out of memory *)
-Defined.
+(* Definition within_err_ub_oom_MemPropT {MemState} {A} (m : MemPropT MemState A) (pre : MemState) (e : err_ub_oom A) (post : MemState) : Prop := *)
+(*     m pre (a <- e;; ret (post, a)). *)
 
-#[global] Instance MemPropT_RAISE_ERROR {MemState : Type} : RAISE_ERROR (MemPropT MemState).
-Proof.
-  split.
-  - intros A msg.
-    unfold MemPropT.
-    intros ms res.
-    destruct res as [[[[[[[oom_res] | [[ub_res] | [[err_res] | [ms' a]]]]]]]]] eqn:Hres.
-    + (* OOM *)
-      exact False. (* Must error *)
-    + (* UB *)
-      exact False. (* Must error *)
-    + (* Error *)
-      exact True. (* Any error message is good *)
-    + (* Success *)
-      exact False. (* Must error. *)
-Defined.
+(* Lemma within_err_ub_oom_MemPropT_eq1Proper {MemState} {A} : *)
+(*   Proper (eq1 ==> eq ==> eq ==> eq ==> iff) (@within_err_ub_oom_MemPropT MemState A). *)
+(* Proof. *)
+(*   unfold Proper, respectful. *)
+(*   intros m1 m2 M x y X b1 b2 B z w Z. *)
+(*   subst. *)
 
-#[global] Instance MemPropT_RAISE_UB {MemState : Type} : RAISE_UB (MemPropT MemState).
-Proof.
-  split.
-  intros A ub_msg.
-    intros ms res.
-    destruct res as [[[[[[[oom_res] | [[ub_res] | [[err_res] | [ms' a]]]]]]]]] eqn:Hres.
-    + (* OOM *)
-      exact False. (* Must UB *)
-    + (* UB *)
-      exact True. (* Any UB message is good *)
-    + (* Error *)
-      exact False. (* Must UB *)
-    + (* Success *)
-      exact False. (* Must UB *)
-Defined.
+(*   unfold within_err_ub_oom_MemPropT. *)
 
-Definition within_err_ub_oom_MemPropT {MemState} {A} (m : MemPropT MemState A) (pre : MemState) (e : err_ub_oom A) (post : MemState) : Prop :=
-    m pre (a <- e;; ret (post, a)).
+(*   split; intros WITHIN; *)
+(*     apply M in WITHIN; auto. *)
+(* Qed. *)
 
-Lemma within_err_ub_oom_MemPropT_eq1Proper {MemState} {A} :
-  Proper (eq1 ==> eq ==> eq ==> eq ==> iff) (@within_err_ub_oom_MemPropT MemState A).
-Proof.
-  unfold Proper, respectful.
-  intros m1 m2 M x y X b1 b2 B z w Z.
-  subst.
+(* #[global] Instance Within_err_ub_oom_MemPropT {MemState} : @Within (MemPropT MemState) _ err_ub_oom MemState MemState := *)
+(*   { *)
+(*     within := @within_err_ub_oom_MemPropT MemState; *)
+(*     within_eq1_Proper := @within_err_ub_oom_MemPropT_eq1Proper MemState; *)
+(*   }. *)
 
-  unfold within_err_ub_oom_MemPropT.
+(* #[global] Instance Within_ret_inv_MemPropT {MemState} {IMS : Inhabited MemState} : *)
+(*   Within_ret_inv (MemPropT MemState) err_ub_oom MemState MemState. *)
+(* Proof. *)
+(*   split. *)
+(*   - intros A x y H. *)
+(*     cbn in *. *)
+(*     firstorder. *)
+(*   - intros A x. *)
+(*     cbn. *)
+(*     inv IMS. *)
+(*     exists inhabitant. exists inhabitant. *)
+(*     auto. *)
+(* Defined. *)
 
-  split; intros WITHIN;
-    apply M in WITHIN; auto.
-Qed.
+(* #[global] Instance Within_ret_pre_post_inv_MemPropT {MemState} : *)
+(*   Within_ret_pre_post_inv (MemPropT MemState) err_ub_oom MemState. *)
+(* Proof. *)
+(*   split. *)
+(*   - intros A pre post x y H. *)
+(*     cbn in *. *)
+(*     firstorder. *)
+(*   - intros A pre x. *)
+(*     cbn. *)
+(*     auto. *)
+(*   - intros A pre1 post1 pre2 post2 x y z w H H0. *)
+(*     cbn in *. *)
+(*     tauto. *)
+(* Defined. *)
 
-#[global] Instance Within_err_ub_oom_MemPropT {MemState} : @Within (MemPropT MemState) _ err_ub_oom MemState MemState :=
-  {
-    within := @within_err_ub_oom_MemPropT MemState;
-    within_eq1_Proper := @within_err_ub_oom_MemPropT_eq1Proper MemState;
-  }.
+(* #[global] Instance RaiseBindM_OOM_MemPropT {MemState} {IMS : Inhabited MemState} : *)
+(*   RaiseBindM (MemPropT MemState) string (@raise_oom (MemPropT MemState) MemPropT_RAISE_OOM). *)
+(* Proof. *)
+(*   split. *)
+(*   - intros A B f x. *)
+(*     cbn. *)
+(*     intros ms e. *)
+(*     destruct e as [[[[[[[oom_e] | [[ub_e] | [[err_e] | [ms' b]]]]]]]]] eqn:He; *)
+(*       firstorder. *)
+(*   - intros A x y CONTRA. *)
+(*     inv IMS. *)
+(*     rename inhabitant into ms. *)
+(*     specialize (CONTRA ms (raise_oom x)). *)
+(*     cbn in *. *)
+(*     tauto. *)
+(* Defined. *)
 
-#[global] Instance Within_ret_inv_MemPropT {MemState} {IMS : Inhabited MemState} :
-  Within_ret_inv (MemPropT MemState) err_ub_oom MemState MemState.
-Proof.
-  split.
-  - intros A x y H.
-    cbn in *.
-    firstorder.
-  - intros A x.
-    cbn.
-    inv IMS.
-    exists inhabitant. exists inhabitant.
-    auto.
-Defined.
+(* #[global] Instance RaiseBindM_ERROR_MemPropT {MemState} {IMS : Inhabited MemState} : *)
+(*   RaiseBindM (MemPropT MemState) string (@raise_error (MemPropT MemState) MemPropT_RAISE_ERROR). *)
+(* Proof. *)
+(*   split. *)
+(*   - intros A B f x. *)
+(*     cbn. *)
+(*     intros ms e. *)
+(*     destruct e as [[[[[[[oom_e] | [[ub_e] | [[err_e] | [ms' b]]]]]]]]] eqn:He; *)
+(*       firstorder. *)
+(*   - intros A x y CONTRA. *)
+(*     inv IMS. *)
+(*     rename inhabitant into ms. *)
+(*     specialize (CONTRA ms (raise_error x)). *)
+(*     cbn in *. *)
+(*     tauto. *)
+(* Defined. *)
 
-#[global] Instance Within_ret_pre_post_inv_MemPropT {MemState} :
-  Within_ret_pre_post_inv (MemPropT MemState) err_ub_oom MemState.
-Proof.
-  split.
-  - intros A pre post x y H.
-    cbn in *.
-    firstorder.
-  - intros A pre x.
-    cbn.
-    auto.
-  - intros A pre1 post1 pre2 post2 x y z w H H0.
-    cbn in *.
-    tauto.
-Defined.
+(* #[global] Instance RaiseWithin_OOM_MemPropT {MemState} : *)
+(*   RaiseWithin (MemPropT MemState) err_ub_oom MemState MemState string *)
+(*     (@raise_oom (MemPropT MemState) MemPropT_RAISE_OOM). *)
+(* Proof. *)
+(*   split. *)
+(*   intros X msg x. *)
+(*   cbn. *)
+(*   intros [ms [ms' CONTRA]]. *)
+(*   auto. *)
+(* Defined. *)
 
-#[global] Instance RaiseBindM_OOM_MemPropT {MemState} {IMS : Inhabited MemState} :
-  RaiseBindM (MemPropT MemState) string (@raise_oom (MemPropT MemState) MemPropT_RAISE_OOM).
-Proof.
-  split.
-  - intros A B f x.
-    cbn.
-    intros ms e.
-    destruct e as [[[[[[[oom_e] | [[ub_e] | [[err_e] | [ms' b]]]]]]]]] eqn:He;
-      firstorder.
-  - intros A x y CONTRA.
-    inv IMS.
-    rename inhabitant into ms.
-    specialize (CONTRA ms (raise_oom x)).
-    cbn in *.
-    tauto.
-Defined.
+(* #[global] Instance RaiseWithin_ERROR_MemPropT {MemState} : *)
+(*   RaiseWithin (MemPropT MemState) err_ub_oom MemState MemState string *)
+(*     (@raise_error (MemPropT MemState) MemPropT_RAISE_ERROR). *)
+(* Proof. *)
+(*   split. *)
+(*   intros X msg x. *)
+(*   cbn. *)
+(*   intros [ms [ms' CONTRA]]. *)
+(*   auto. *)
+(* Defined. *)
 
-#[global] Instance RaiseBindM_ERROR_MemPropT {MemState} {IMS : Inhabited MemState} :
-  RaiseBindM (MemPropT MemState) string (@raise_error (MemPropT MemState) MemPropT_RAISE_ERROR).
-Proof.
-  split.
-  - intros A B f x.
-    cbn.
-    intros ms e.
-    destruct e as [[[[[[[oom_e] | [[ub_e] | [[err_e] | [ms' b]]]]]]]]] eqn:He;
-      firstorder.
-  - intros A x y CONTRA.
-    inv IMS.
-    rename inhabitant into ms.
-    specialize (CONTRA ms (raise_error x)).
-    cbn in *.
-    tauto.
-Defined.
+(* #[global] Instance RetWithin_UB_MemPropT {MemState} : *)
+(*   RetWithin (MemPropT MemState) err_ub_oom MemState MemState string *)
+(*     (@raise_ub err_ub_oom RAISE_UB_err_ub_oom_T). *)
+(* Proof. *)
+(*   split. *)
+(*   intros X msg x. *)
+(*   cbn. *)
+(*   intros [ms [ms' CONTRA]]. *)
+(*   auto. *)
+(* Defined. *)
 
-#[global] Instance RaiseWithin_OOM_MemPropT {MemState} :
-  RaiseWithin (MemPropT MemState) err_ub_oom MemState MemState string
-    (@raise_oom (MemPropT MemState) MemPropT_RAISE_OOM).
-Proof.
-  split.
-  intros X msg x.
-  cbn.
-  intros [ms [ms' CONTRA]].
-  auto.
-Defined.
+(* #[global] Instance RetInvWithin_MemPropT {MemState} : *)
+(*   RetInvWithin (MemPropT MemState) err_ub_oom MemState MemState. *)
+(* Proof. *)
+(*   split. *)
+(*   intros X msg x. *)
+(*   cbn. *)
+(*   intros [ms [ms' CONTRA]]. *)
+(*   auto. *)
+(*   break_match_hyp. *)
+(*   break_match_hyp. *)
+(*   break_match_hyp. *)
+(*   break_match_hyp. *)
+(*   break_match_hyp. *)
+(*   break_match_hyp. *)
+(*   break_match_hyp; inv CONTRA. *)
+(*   break_match_hyp. *)
+(*   break_match_hyp; inv CONTRA. *)
+(*   break_match_hyp. *)
+(*   break_match_hyp; inv CONTRA. *)
+(*   destruct p. *)
+(*   destruct CONTRA; subst. *)
+(*   destruct_err_ub_oom msg; cbn in *; inv Heqe. *)
+(*   auto. *)
+(* Defined. *)
 
-#[global] Instance RaiseWithin_ERROR_MemPropT {MemState} :
-  RaiseWithin (MemPropT MemState) err_ub_oom MemState MemState string
-    (@raise_error (MemPropT MemState) MemPropT_RAISE_ERROR).
-Proof.
-  split.
-  intros X msg x.
-  cbn.
-  intros [ms [ms' CONTRA]].
-  auto.
-Defined.
+(* #[global] Instance DisjointRaiseWithin_UB_MemPropT {MemState} : *)
+(*   DisjointRaiseWithin (MemPropT MemState) err_ub_oom MemState MemState string *)
+(*     (@raise_ub err_ub_oom RAISE_UB_err_ub_oom_T) (@raise_oom (MemPropT MemState) MemPropT_RAISE_OOM). *)
+(* Proof. *)
+(*   split. *)
+(*   intros X msg1 msg2. *)
+(*   cbn. *)
+(*   intros [ms [ms' CONTRA]]. *)
+(*   auto. *)
+(* Defined. *)
 
-#[global] Instance RetWithin_UB_MemPropT {MemState} :
-  RetWithin (MemPropT MemState) err_ub_oom MemState MemState string
-    (@raise_ub err_ub_oom RAISE_UB_err_ub_oom_T).
-Proof.
-  split.
-  intros X msg x.
-  cbn.
-  intros [ms [ms' CONTRA]].
-  auto.
-Defined.
+(* #[global] Instance MemPropT_Eq1_ret_inv {MemState} `{IMS : Inhabited MemState} : Eq1_ret_inv (MemPropT MemState). *)
+(* Proof. *)
+(*   split. *)
+(*   intros A x y EQ. *)
+(*   cbn in EQ. *)
+(*   red in EQ. *)
+(*   red in EQ. *)
+(*   inversion IMS. *)
+(*   rename inhabitant into initial_memory_state. *)
+(*   specialize (EQ initial_memory_state (ret (initial_memory_state, x))). *)
+(*   cbn in *. *)
+(*   tauto. *)
+(* Defined. *)
 
-#[global] Instance RetInvWithin_MemPropT {MemState} :
-  RetInvWithin (MemPropT MemState) err_ub_oom MemState MemState.
-Proof.
-  split.
-  intros X msg x.
-  cbn.
-  intros [ms [ms' CONTRA]].
-  auto.
-  break_match_hyp.
-  break_match_hyp.
-  break_match_hyp.
-  break_match_hyp.
-  break_match_hyp.
-  break_match_hyp.
-  break_match_hyp; inv CONTRA.
-  break_match_hyp.
-  break_match_hyp; inv CONTRA.
-  break_match_hyp.
-  break_match_hyp; inv CONTRA.
-  destruct p.
-  destruct CONTRA; subst.
-  destruct_err_ub_oom msg; cbn in *; inv Heqe.
-  auto.
-Defined.
-
-#[global] Instance DisjointRaiseWithin_UB_MemPropT {MemState} :
-  DisjointRaiseWithin (MemPropT MemState) err_ub_oom MemState MemState string
-    (@raise_ub err_ub_oom RAISE_UB_err_ub_oom_T) (@raise_oom (MemPropT MemState) MemPropT_RAISE_OOM).
-Proof.
-  split.
-  intros X msg1 msg2.
-  cbn.
-  intros [ms [ms' CONTRA]].
-  auto.
-Defined.
-
-#[global] Instance MemPropT_Eq1_ret_inv {MemState} `{IMS : Inhabited MemState} : Eq1_ret_inv (MemPropT MemState).
-Proof.
-  split.
-  intros A x y EQ.
-  cbn in EQ.
-  red in EQ.
-  red in EQ.
-  inversion IMS.
-  rename inhabitant into initial_memory_state.
-  specialize (EQ initial_memory_state (ret (initial_memory_state, x))).
-  cbn in *.
-  tauto.
-Defined.
-
-Definition MemPropT_assert_pre {MemState} (assertion : Prop) : MemPropT MemState unit
-  := fun ms ms'x =>
-       match ms'x with
-       | ERR_UB_OOM (mkEitherT (mkEitherT (mkEitherT (mkIdent ms'x)))) =>
-           match ms'x with
-           | inl (OOM_message x) =>
-               False
-           | inr (inl (UB_message x)) =>
-               ~ assertion
-           | inr (inr (inl (ERR_message x))) =>
-               False
-           | inr (inr (inr (ms',x))) =>
-               ms = ms' /\ assertion
-           end
-       end.
+(* Definition MemPropT_assert_pre {MemState} (assertion : Prop) : MemPropT MemState unit *)
+(*   := fun ms ms'x => *)
+(*        match ms'x with *)
+(*        | ERR_UB_OOM (mkEitherT (mkEitherT (mkEitherT (mkIdent ms'x)))) => *)
+(*            match ms'x with *)
+(*            | inl (OOM_message x) => *)
+(*                False *)
+(*            | inr (inl (UB_message x)) => *)
+(*                ~ assertion *)
+(*            | inr (inr (inl (ERR_message x))) => *)
+(*                False *)
+(*            | inr (inr (inr (ms',x))) => *)
+(*                ms = ms' /\ assertion *)
+(*            end *)
+(*        end. *)
 
 Definition MemPropT_lift_PropT {MemState X} {E} `{UBE -< E} `{OOME -< E} `{FailureE -< E} (spec : MemPropT MemState X) :
   stateT MemState (PropT E) X.
